added wp

assignment1/WeakestPrecondition/submission.dfy
@@ -1,7 +1,7 @@
 // Please, before you do anything else, add your names here:
 // Group:    69
 // Member 1: Dominika Orzechowska: 2098199
-// Member 2: <Full name 2>: <Student number 2>
+//  Member 2:  Jort Kuipers 2111446
 
 include "assignment.dfy" 
 
@@ -12,13 +12,22 @@ module Submission refines Assignment {
         x < 9  && (x <= 0 ==> |a| > 0 && a[0] < 10)
     }
 
-    ghost predicate precon1(x: int)
+    ghost predicate precon1(x: int) {
+        !(x < 10) &&
+        ((x < 10) ==> (((x<20) ==> 1 % 2 == 0) && (!(x<20) ==> 2 % 2 == 0) )) && ((!(x < 10) ==> (4 % 2 == 0)))
+    }
 
-    ghost predicate precon2(x: int)
+    ghost predicate precon2(x: int){
+        ((x < 8)==> ((x < 4) ==> (x + 1) % 2 == 0) ) && ( (x < 8) ==> (!(x < 4) ==> 2 % 2 ==0) ) && ( !(x < 8) ==> ( (x + 2) % 2 == 0 && ( (x < 32) ==> (1 % 2 ==0) ) ) )
+    }
 
-    ghost predicate precon3(x: int)
+    ghost predicate precon3(x: int){
+        x == 2 || (34 <= x < 55)
+    }
 
-    ghost predicate precon4(u: int, a: seq<int>)
+    ghost predicate precon4(u: int, a: seq<int>){
+        (0 <= u+1 < |a|) && (a[u+1] % 2 == 0) 
+    }
     
     // example
     method precon0_calc(x: int, a: seq<int>) returns (y: int)
@@ -43,14 +52,19 @@ module Submission refines Assignment {
     method precon1_calc(x: int) returns (y: int)
       requires precon1(x) 
     {
+        assert !(x < 10);
+        assert ((x < 10) ==> (((x<20) ==> 1 % 2 == 0) && (!(x<20) ==> 2 % 2 == 0) )) && ((!(x < 10) ==> (4 % 2 == 0)));
         if x < 10 {
+            assert false;
             if x < 20 {
                 y := 1;
             } else {
-                y := 2;
+                y := 2; 
+                assert y == 2 * 1;
             }
         } else {
             y := 4;
+            assert y == 2 * 2;
         }
         assert y % 2 == 0; 
     }
@@ -58,13 +72,20 @@ module Submission refines Assignment {
     method precon2_calc(x: int) returns (y: int, z: int)
         requires precon2(x)
     {
+        assert ((x < 8)==> ((x < 4) ==> (x + 1) % 2 == 0) ) && ( (x < 8) ==> (!(x < 4) ==> 2 % 2 ==0) ) && ( !(x < 8) ==> ( (x + 2) % 2 == 0 && ( (x < 32) ==> (1 % 2 ==0) ) ) );
+        
         z := 0;
         if x < 8 {
+            assert (x < 4) ==> (x + 1) % 2 == 0 && (!(x < 4) ==> 2 % 2 ==0);
             if x < 4 {
+                assert x < 4;
+                assert (x + 1) % 2 == 0;
                 z := x + 1;
                 y := z;
+                assert y % 2 == 0;
             } else {
                 y := 2;
+                assert y % 2 == 0;
             }
         } else {
             y := x + 2;
@@ -78,16 +99,24 @@ module Submission refines Assignment {
     method precon3_calc(x: int) returns (y: int)
         requires precon3(x)
     {
+        assert x == 2 || (34 <= x < 55);
+        assert (x == 2 ==> (0 <= x + 1 < 100)) && ((34 <= x < 55) ==> (0 <= 21 < 100));
         if x < 34 {
             if x == 2 {
+                assert x == 2;
                 y := x + 1;
+                assert 0 <= y < 100;
+
             } else {
+                assert false;
                 y := 233;
             }
         } else {
             if x < 55 {
                 y := 21;
+                assert 0 <= y < 100;
             } else {
+                assert false;
                 y := 144;
             }
         }
@@ -97,8 +126,10 @@ module Submission refines Assignment {
     method precon4_calc(u: int, a: seq<int>) returns (t: int)
         requires precon4(u, a)
     {
+        assert (0 <= u+1 < |a|) && (a[u+1] % 2 == 0); 
         t := a[u+1];
         t := t + 4;
         assert t % 2 == 0;
     }
+
 }
